added register to enrollStation

tokeneer/token.dfy
@@ -2,23 +2,26 @@ datatype clearanceLevel = Low | Medium | High
 
 class Token {
 
-    var valifyer : bool
-	var security_level : clearanceLevel;
-	var user_ID	: int
+    var valifyer : bool;
+	var clearance_level : clearanceLevel;
+	var user_ID	: int;
 	
 
 
-constructor (id : int, sec_lvl : clearanceLevel)
+method INIT (id : int, sec_lvl : clearanceLevel)
+modifies this`valifyer
+modifies this`user_ID
+modifies this`clearance_level
 requires id >= 0 	// users always a positive integer
 ensures 		valifyer 
 			&&  user_ID == id 
-			&&  security_level == sec_lvl
+			&&  clearance_level == sec_lvl
 {
-
-valifyer := true;
-security_level := sec_lvl;
+clearance_level := sec_lvl;
 user_ID := id;
+valifyer := true;
 }
+
 
 
 /*
@@ -28,12 +31,11 @@ ensures  : that the current token is invalid
 
 method invalidateToken()
 modifies this`valifyer
-requires valifyer == true
-ensures valifyer == false 
+requires  valifyer
+ensures  !valifyer 
 {
 
 valifyer := false;
-
 }
 
 }
@@ -45,49 +47,69 @@ valifyer := false;
 
 
 class User{
-	var user_ID  	: int 
 	var token 		: Token
 
-	constructor(uID : int)
-    requires uID > 0
-	 ensures uID == uID
+	method INIT()
+	modifies this`token
+	ensures token == null	
 	{
-		user_ID := uID;
-	}
-
-/*
-	method enroll()
-	requires token != null
-	ensures token.user_ID == user_ID
-	{
-
-*/
-
+		token := null;
 
 	}
 
+
+	}
 
 
 //================================= Class Enrolmmentsys  ===========================================
 
 
 class EnrollmentSystem{
-  var maxUsers : int;
-  var userMap : map< int, Token>;
 
-	constructor(maxU : int)
-  requires maxUsers > 0
-  ensures maxUsers == maxU
-  ensures |userMap| == 0
-  {
-    maxUsers := maxU;
-    userMap :=map[];
-  }
+var idCounter : int;
+var userSet : set<int>;
 
+predicate Valid_Enrollment()
+reads this`idCounter
+reads this`userSet
+{
+	 0 <= idCounter 
 
 }
 
 
+method INIT()
+	modifies this`idCounter
+	modifies this`userSet
+		ensures userSet == {} && |userSet| == 0 
+		ensures idCounter == 0 
+  {
+    userSet := {};
+    idCounter := 0;
+  }
+
+method register(user : User, cl : clearanceLevel)
+	modifies this`userSet
+	modifies this`idCounter
+	modifies user`token, user.token
+		requires user != null
+		requires 	Valid_Enrollment()
+		ensures 	Valid_Enrollment()
+		ensures old(idCounter)  == idCounter - 1 
+		{
+
+			userSet := userSet + {idCounter};
+			// write method for this
+			user.token  := new Token.INIT(idCounter, cl);
+			idCounter := idCounter + 1;
+
+		}
+
+
+
+
+
+}
 
 
 
